src/coq/Semantics/Memory/ErrSID.v
@@ -36,41 +36,49 @@ Module ERRSID (Addr:ADDRESS) (IP:INTPTR) (SIZEOF:Sizeof) (LLVMEvents:LLVM_INTERA
   Import PROV.
 
   (* Need failure, UB, state for store_ids, and state for provenances *)
-  Definition ErrSID_T M := eitherT ERR_MESSAGE (eitherT UB_MESSAGE (stateT store_id (stateT Provenance M))).
+  Definition ErrSID_T M := eitherT ERR_MESSAGE (eitherT UB_MESSAGE (eitherT OOM_MESSAGE (stateT store_id (stateT Provenance M)))).
   Definition ErrSID := ErrSID_T ident.
 
   (* I can make this work using ltac, but  for some reason I can't write the definition directly... *)
   #[global] Instance ErrSID_T_MT {M : Type -> Type} `{HM: Monad M} : MonadT (ErrSID_T M) M.
   Proof.
     constructor.
-    refine (fun T mt => mkEitherT (mkEitherT (fun sid prov => _))).
-    refine (fmap (fun v => (prov, (sid, inr (inr v)))) mt : M (Provenance * (store_id * UB (ERR T)))%type).
+    refine (fun T mt => mkEitherT (mkEitherT (mkEitherT (fun sid prov => _)))).
+    refine (fmap (fun v => (prov, (sid, inr (inr (inr v))))) mt : M (Provenance * (store_id * (OOM_MESSAGE + UB (ERR T))))%type).
   Defined.
 
   #[global] Instance RAISE_UB_ErrSID_T {M : Type -> Type} `{HM :  Monad M} : RAISE_UB (ErrSID_T M) :=
     { raise_ub := fun A e => lift (raise_ub e);
     }.
 
-  Definition evalErrSID_T {A} {M} `{Monad M} (m : ErrSID_T M A) (sid : store_id) (prov : Provenance) : M (UB (ERR A))
-    := evalStateT (evalStateT (unEitherT (unEitherT m)) sid) prov.
+  #[global] Instance RAISE_ERROR_ErrSID_T {M : Type -> Type} `{HM :  Monad M} : RAISE_ERROR (ErrSID_T M) :=
+    { raise_error := fun A e => raise_error e;
+    }.
 
-  Definition evalErrSID {A} (m : ErrSID A) (sid : store_id) (prov : Provenance) : UB (ERR A)
+  #[global] Instance RAISE_OOM_ErrSID_T {M : Type -> Type} `{HM :  Monad M} : RAISE_OOM (ErrSID_T M) :=
+    { raise_oom := fun A e => lift (lift (raise_oom e));
+    }.
+
+  Definition evalErrSID_T {A} {M} `{Monad M} (m : ErrSID_T M A) (sid : store_id) (prov : Provenance) : M (OOM_MESSAGE + UB (ERR A))%type
+    := evalStateT (evalStateT (unEitherT (unEitherT (unEitherT m))) sid) prov.
+
+  Definition evalErrSID {A} (m : ErrSID A) (sid : store_id) (prov : Provenance) : OOM_MESSAGE + UB (ERR A)
     := unIdent (evalErrSID_T m sid prov).
 
-  Definition runErrSID_T {A} {M} `{Monad M} (m : ErrSID_T M A) (sid : store_id) (prov : Provenance) : M (UB (ERR A) * store_id * Provenance)%type
-    := runStateT (runStateT (unEitherT (unEitherT m)) sid) prov.
+  Definition runErrSID_T {A} {M} `{Monad M} (m : ErrSID_T M A) (sid : store_id) (prov : Provenance) : M ((OOM_MESSAGE + UB (ERR A)) * store_id * Provenance)%type
+    := runStateT (runStateT (unEitherT (unEitherT (unEitherT m))) sid) prov.
 
-  Definition runErrSID {A} (m : ErrSID A) (sid : store_id) (prov : Provenance) : UB (ERR A) * store_id * Provenance%type
+  Definition runErrSID {A} (m : ErrSID A) (sid : store_id) (prov : Provenance) : (OOM_MESSAGE + UB (ERR A)) * store_id * Provenance%type
     := unIdent (runErrSID_T m sid prov).
 
   Definition ErrSID_evals_to {A} (e : ErrSID A) (x : A) sid pr : Prop
-    := evalErrSID e sid pr = inr (inr x).
+    := evalErrSID e sid pr = inr (inr (inr x)).
 
   Definition fresh_sid : ErrSID store_id
     := lift (lift (modify N.succ)).
 
   Definition fresh_provenance : ErrSID Provenance
-    := lift (lift (lift (modify next_provenance))).
+    := lift (lift (lift (lift (modify next_provenance)))).
 
   Definition fresh_allocation_id : ErrSID AllocationId
     := prov <- fresh_provenance;;
@@ -79,8 +87,7 @@ Module ERRSID (Addr:ADDRESS) (IP:INTPTR) (SIZEOF:Sizeof) (LLVMEvents:LLVM_INTERA
   Definition err_to_ub {A} (e : err A) : ErrSID A
     := match e with
        | inl msg =>
-         (* TODO: can this be inferred...? *)
-         @raise_ub ErrSID (@RAISE_UB_E_MT _ _ _ (@RAISE_UB_MonadExc (eitherT UB_MESSAGE (stateT store_id (stateT Provenance ident))) _)) _ msg
+           raise_ub msg
        | inr x => ret x
        end.
 
