src/coq/Handlers/Local.v
@@ -170,7 +170,7 @@ From Vellvm Require Import
    it until [TopLevel] either.
    So exposing the specialization here, but it is awkward.
  *)
-Module Make (A : ADDRESS)(SIZEOF : Sizeof)(LLVMEvents : LLVM_INTERACTIONS(A)(SIZEOF)).
+Module Make (A : ADDRESS)(IP : INTPTR)(SIZEOF : Sizeof)(LLVMEvents : LLVM_INTERACTIONS(A)(IP)(SIZEOF)).
   Definition local_env := FMapAList.alist raw_id LLVMEvents.DV.uvalue.
 End Make.
 
